AwsCryptographicMaterialProviders/dafny/AwsCryptographyKeyStoreAdmin/src/MutationStateStructures.dfy
@@ -13,6 +13,7 @@ include "MutationIndexUtils.dfy"
 module {:options "/functionSyntax:4" } MutationStateStructures {
   import opened StandardLibrary
   import opened StandardLibrary.UInt
+  import opened StandardLibrary.NeedError
   import opened Wrappers
   import opened Seq
   import UTF8
@@ -72,6 +73,17 @@ module {:options "/functionSyntax:4" } MutationStateStructures {
     CommitmentCiphertext: seq<uint8>,
     IndexCiphertext: seq<uint8>
   )
+  {
+    ghost predicate ValidState()
+    {
+      && 0 < |Identifier|
+      && 0 < |UUID|
+      && KmsArn.ValidKmsArn?(Original.kmsArn)
+      && KmsArn.ValidKmsArn?(Terminal.kmsArn)
+      && (Structure.BRANCH_KEY_RESTRICTED_FIELD_NAMES !! Original.customEncryptionContext.Keys)
+      && (Structure.BRANCH_KEY_RESTRICTED_FIELD_NAMES !! Terminal.customEncryptionContext.Keys)
+    }
+  }
 
   /** The Commitment & Index are persisted to the storage by Initialize. **/
   /** The Commitment & Index are read by Apply. **/
@@ -84,20 +96,26 @@ module {:options "/functionSyntax:4" } MutationStateStructures {
   {
     /** The Commitment & Index MUST always have the same Identifier & UUID. **/
     /** They MAY NOT have the same CreateTime. **/
-    ghost predicate ValidState()
+    predicate ValidState()
     {
       && Commitment.Identifier == Index.Identifier
+      && 0 < |Commitment.Identifier|
       && Commitment.UUID == Index.UUID
+      && 0 < |Commitment.UUID|
+    }
+    predicate ValidUTF8()
+    {
+      && UTF8.ValidUTF8Seq(Commitment.Original)
+      && UTF8.ValidUTF8Seq(Commitment.Terminal)
+      && UTF8.ValidUTF8Seq(Commitment.Input)
+      && UTF8.ValidUTF8Seq(Index.PageIndex)
+      && 0 < |Commitment.Identifier|
+      && 0 < |Index.Identifier|
+      && 0 < |Commitment.UUID|
+      && 0 < |Index.UUID|
     }
   }
 
-  predicate MutationToApply?(MutationToApply: MutationToApply)
-  {
-    && KmsArn.ValidKmsArn?(MutationToApply.Original.kmsArn)
-    && KmsArn.ValidKmsArn?(MutationToApply.Terminal.kmsArn)
-    && (Structure.BRANCH_KEY_RESTRICTED_FIELD_NAMES !! MutationToApply.Original.customEncryptionContext.Keys)
-    && (Structure.BRANCH_KEY_RESTRICTED_FIELD_NAMES !! MutationToApply.Terminal.customEncryptionContext.Keys)
-  }
 
   function EncryptionContextStringToJSON(
     encryptionContext: KeyStoreTypes.EncryptionContextString
@@ -137,29 +155,6 @@ module {:options "/functionSyntax:4" } MutationStateStructures {
   ): (output: Result<JSONValues.JSON, Types.Error>)
   {
     Success(JSONValues.JSON.String(kmsArn))
-  }
-
-  function NeedOutcome<E>(
-    condition: bool,
-    error: () --> E)
-    : (result: Outcome2<E>)
-    requires !condition ==> error.requires()
-  {
-    if condition then Outcome2.Pass else Outcome2.Fail(error())
-  }
-
-  datatype Outcome2<E> = Pass | Fail(error: E)
-  {
-    predicate IsFailure() {
-      Fail?
-    }
-    // Note: PropagateFailure returns a Result, not an Outcome.
-    function PropagateFailure(): Outcome<E>
-      requires Fail?
-    {
-      Outcome.Fail(this.error)
-    }
-    // Note: no Extract method
   }
 
   function InputMutationsToJson(
@@ -216,10 +211,32 @@ module {:options "/functionSyntax:4" } MutationStateStructures {
     Success(input)
   }
 
+  function ValidateJSONSerialize(
+    jsonByteSeq: seq<uint8>
+  ): (output: Result<UTF8.ValidUTF8Bytes, string>)
+    ensures
+      output.Success?
+      ==>
+        && UTF8.ValidUTF8Seq(jsonByteSeq)
+        && output.value == jsonByteSeq
+  {
+    if UTF8.ValidUTF8Seq(jsonByteSeq)
+    then Success(jsonByteSeq)
+    else Failure("Failure to UTF8 Validate results of JSON Serialization.")
+  }
+
   function SerializeMutationCommitment(
     MutationToApply: MutationToApply
   ): (output: Result<KeyStoreTypes.MutationCommitment, Types.Error>)
-    requires MutationToApply?(MutationToApply)
+    requires MutationToApply.ValidState() //MutationToApply?(MutationToApply)
+    ensures
+      && output.Success?
+      ==>
+        && UTF8.ValidUTF8Seq(output.value.Original)
+        && UTF8.ValidUTF8Seq(output.value.Terminal)
+        && UTF8.ValidUTF8Seq(output.value.Input)
+        && 0 < |output.value.Identifier|
+        && 0 < |output.value.UUID|
   {
     var OriginalJson
       := JSONValues.Object(
@@ -239,23 +256,38 @@ module {:options "/functionSyntax:4" } MutationStateStructures {
     var originalBytes :- JSON.Serialize(OriginalJson).MapFailure(
                            (e: JSONErrors.SerializationError)
                            => Types.KeyStoreAdminException(
-                               message := "Could not JSON Serialize state: original properties. " + e.ToString()));
+                               message := "Could not JSON Serialize original properties. " + e.ToString()));
+    var validatedOriginalBytes: UTF8.ValidUTF8Bytes :- ValidateJSONSerialize(originalBytes)
+                                                       .MapFailure(
+                                                         (e: string) =>
+                                                           Types.KeyStoreAdminException(message := "Could not JSON Serialize original properties. " + e));
+
     var terminalBytes :- JSON.Serialize(TerminalJson).MapFailure(
                            (e: JSONErrors.SerializationError)
                            => Types.KeyStoreAdminException(
-                               message := "Could not JSON Serialize state: terminal properties. " + e.ToString()));
+                               message := "Could not JSON Serialize terminal properties. " + e.ToString()));
+    var validatedTerminalBytes: UTF8.ValidUTF8Bytes :- ValidateJSONSerialize(terminalBytes)
+                                                       .MapFailure(
+                                                         (e: string) =>
+                                                           Types.KeyStoreAdminException(message := "Could not JSON Serialize terminal properties. " + e));
+
     var inputBytes :- JSON.Serialize(InputJson).MapFailure(
                         (e: JSONErrors.SerializationError)
                         => Types.KeyStoreAdminException(
                             message := "Could not JSON Serialize Input. " + e.ToString()));
+    var validatedInputBytes: UTF8.ValidUTF8Bytes :- ValidateJSONSerialize(inputBytes)
+                                                    .MapFailure(
+                                                      (e: string) =>
+                                                        Types.KeyStoreAdminException(message := "Could not JSON Serialize Input. " + e));
+
     var commitment := KeyStoreTypes.MutationCommitment(
                         Identifier := MutationToApply.Identifier,
-                        Original := originalBytes,
-                        Terminal := terminalBytes,
+                        Original := validatedOriginalBytes, //originalBytes,
+                        Terminal := validatedTerminalBytes, //terminalBytes,
                         UUID := MutationToApply.UUID,
                         CreateTime := MutationToApply.CreateTime,
                         CiphertextBlob := MutationToApply.CommitmentCiphertext,
-                        Input := inputBytes
+                        Input := validatedInputBytes //inputBytes
                       );
     Success(commitment)
   }
@@ -264,7 +296,13 @@ module {:options "/functionSyntax:4" } MutationStateStructures {
     MutationToApply: MutationToApply,
     ExclusiveStartKey: MutationIndexUtils.ExclusiveStartKey
   ): (output: Result<KeyStoreTypes.MutationIndex, Types.Error>)
-    requires MutationToApply?(MutationToApply)
+    requires MutationToApply.ValidState() //MutationToApply?(MutationToApply)
+    ensures
+      && output.Success?
+      ==>
+        && UTF8.ValidUTF8Seq(output.value.PageIndex)
+        && 0 < |output.value.Identifier|
+        && 0 < |output.value.UUID|
   {
     var index := KeyStoreTypes.MutationIndex(
                    Identifier := MutationToApply.Identifier,
@@ -276,10 +314,11 @@ module {:options "/functionSyntax:4" } MutationStateStructures {
     Success(index)
   }
 
-  function DeserializeMutation(
+  function {:isolate_assertions} DeserializeMutation(
     commitmentAndIndex: CommitmentAndIndex
   ): (output: Result<MutationToApply, Types.Error>)
-    ensures output.Success? ==> MutationToApply?(output.value)
+    requires commitmentAndIndex.ValidState()
+    ensures output.Success? ==> output.value.ValidState()
   {
     var commitment := commitmentAndIndex.Commitment;
     var index := commitmentAndIndex.Index;
@@ -301,16 +340,33 @@ module {:options "/functionSyntax:4" } MutationStateStructures {
     :- MutablePropertiesJson?(TerminalJson);
     :- MutationsInputJson?(InputJson);
 
+    :- Need(
+         UTF8.ValidUTF8Seq(index.PageIndex),
+         Types.KeyStoreAdminException(
+           message := "PageIndex (pageIndex) is not a Valid UTF-8 Byte sequence."));
+
+    var OriginalEC := JSONToEncryptionContextString(OriginalJson.obj[0].1);
+    :- Need(
+         Structure.BRANCH_KEY_RESTRICTED_FIELD_NAMES !! OriginalEC.Keys,
+         Types.KeyStoreAdminException(
+           message:="Original Properities contain illegal Encryption Context! There are some resereved Encryption Context Keys!"));
+
+    var TerminalEC := JSONToEncryptionContextString(TerminalJson.obj[0].1);
+    :- Need(
+         Structure.BRANCH_KEY_RESTRICTED_FIELD_NAMES !! TerminalEC.Keys,
+         Types.KeyStoreAdminException(
+           message:="Terminal Properities contain illegal Encryption Context! There are some resereved Encryption Context Keys!"));
+
     Success(
       MutationToApply(
         Identifier := commitment.Identifier,
         Original := MutableProperties(
           kmsArn := OriginalJson.obj[1].1.str,
-          customEncryptionContext := JSONToEncryptionContextString(OriginalJson.obj[0].1)
+          customEncryptionContext := OriginalEC
         ),
         Terminal := MutableProperties(
           kmsArn := TerminalJson.obj[1].1.str,
-          customEncryptionContext := JSONToEncryptionContextString(TerminalJson.obj[0].1)
+          customEncryptionContext := TerminalEC
         ),
         UUID := commitment.UUID,
         CreateTime := commitment.CreateTime,
